已知：

1. $sin\ (\alpha+\beta)=sin\  \alpha \ cos\ \beta -cos\  \alpha \ sin\  \beta= \frac{1}{3}$
2. $cos\  \alpha \ sin\ \ \beta = \frac{1}{6}$  

由(1)得：
$sin\  \alpha \ cos\  \beta = sin\ (\alpha - \beta) + cos\  \alpha \ sin\  \beta = \frac{1}{3} + \frac{1}{6} = \frac{1}{2}$  

这样就得到两个重要结果：

1. $sin\  \alpha \ cos\  \beta = \frac{1}{2}$

2. $cos\  \alpha \ sin\ \ \beta = \frac{1}{6}$

接下来就可以对 $cos\ (2 \alpha + 2 \beta)$ 进行求解了


$\because sin\ (\alpha + \beta) = sin\  \alpha \ cos\  \beta + cos\  \alpha \ sin\  \beta$  
$\therefore sin\ (\alpha + \beta) = \frac{2}{3}$  
$\because 2 \alpha + 2 \beta = 2(\alpha + \beta)$  
$\therefore cos\ (2 \alpha + 2 \beta) = cos\ (2(\alpha + \beta)) = 1 - 2sin^{2}(\alpha + \beta) = 1 - 2 \times (\frac{2}{3})^{2} = \frac{1}{9}$
